**第二章测试**

1. 关于Fibonacci序列，有

$F(1)+F(2)+\ldots+F(n)=F(n+2)-1$

证明：

$F(1)=F(3)-F(2)$

$F(2)=F(4)-F(3)$

$F(3)=F(5)-F(4)$

$\cdots$

$F(n)=F(n+2)-F(n+1)$

上述等式相加，即有：

$F(1)+F(2)+\cdots+F(n)=F(n+2)-F(2)=F(n+2)-1$

2. 求序列$0,1×2×3,2×3×4,\ldots,n(n+1)(n+2),\ldots$的母函数。

$$
\frac{1}{1-x}=1+x+x^2+\ldots
$$

$$
\frac{1}{(1-x)^2}=1+2x+3x^2+\ldots
$$

$$
\frac{2}{(1-x)^3}=2+2×3x+3×4x^2+\ldots
$$

$$
\frac{6}{(1-x)^4}=1×2×3+2×3×4x+\ldots
$$

$$
\frac{6x}{(1-x)^4}=0+1×2×3x+2×3×4x^2+\ldots
$$

则母函数为$\frac{6x}{(1-x)^4}$

3. 求$G(x)=\frac{1}{(1-x)(1-x^2)(1-x^3)}$中$x^n$的系数$a_n$

解：$G(x)=\frac{1}{(1-x)(1-x^2)(1-x^3)}=\frac{1}{(1-x)^3(1+x)(1+x+x^2)}$

其中$(1-x)^3,$三重根$\alpha=1$

$1+x=1-(-x),\alpha=-1$

$1+x+x^2=(x-\frac{-1+\sqrt{3}i}{2})(x-\frac{-1-\sqrt{3}i}{2})=(1-\alpha_1x)(1-\alpha_2x)$，有共轭复根$\alpha_1=\frac{-1-\sqrt{3}i}{2},\alpha_2=\frac{-1-\sqrt{3}i}{2}$，其中$\rho=1,\theta=\frac{2\pi}{3}$

> 有$a_n=A(-1)^n+(B+Cn+Dn^2)1^n+(Ecos\frac{2n\pi}{3}+Fsin\frac{2n\pi}{3})$,但好像$a_0、a_1、a_2、a_3、a_4、a_5$不太好求得，因此换一种方法：

$G(x)=\frac{A}{1+x}+\frac{B}{x-\frac{-1+\sqrt{3}i}{2}}+\frac{C}{x-\frac{-1-\sqrt{3}i}{2}}+\frac{D}{1-x}+\frac{E}{(1-x)^2}+\frac{F}{(1-x)^3}$

求得$A=1/8,B=\frac{1-\sqrt{3}i}{18},C=\frac{1+\sqrt{3}i}{18},D=17/72,E=1/4,F=1/6$

则有$a_n=\frac{1}{8}(-1)^n+\frac{1}{9}(\frac{-1+\sqrt{3}i}{2})^n+\frac{1}{9}(\frac{-1-\sqrt{3}i}{2})^n+\frac{17}{72}+\frac{n+1}{4}+\frac{(n+1)(n+2)}{12}=\frac{1}{8}(-1)^n+\frac{2}{9}\cos\frac{2n\pi}{3}+\frac{17}{72}+\frac{n+1}{4}+\frac{(n+1)(n+2)}{12}$

4. 给出下列序列的母函数

(1) $1,0,1,0,1,0,1,0 \cdots$

$G(x)=1+0x+1x^2+0x^3+1x^4+0x^5+1x^6+0x^7+\cdots$

故它的母函数为： $$ G(x) = 1+x^2+x^4+x^6+\cdots = \frac{1}{1-x^2} $$

(2) $1,-1,1,-1,1,-1,1 \cdots$

$G(x)=1-x+x^2-x^3+x^4-x^5+\cdots$

故它的母函数为： $$ G(x) = 1-x+x^2-x^3+x^4-x^5+\cdots = \frac{1}{1+x} $$

5. 求序列$\{1,0,2,0,3,0,4,0,\cdots\}$的通项公式

解：

$G(x)=1+2x^2+3x^4+4x^6+\cdots=\frac{1}{(1-x^2)^2}=\frac{1}{(1+x)^2(1-x)^2}$

则:$a_n=(An+B)(-1)^n+(Cn+D)$

根据$a_0=1,a_1=0,a_2=2,a_3=0$

可得$A=1/4,B=1/2,C=1/4,D=1/2$

则通项公式为$a_n=\frac{1}{4}(n+2)[1+(-1)^n]$
